\documentclass{article}[12pt]
\usepackage{amsmath}
\input{include.tex}
\input{Definitions.tex}
\begin{document}
\section{Idea of new parameterisation $\mLambda = (\mR^T \mR)^{-1}$}
\begin{equation*}
\frac{\partial \log p(y;\vmu, \mLambda)}{\partial \mLambda_{ij}} = \half \tr ((\mLambda^{-1} - C^T W C - B)\frac{\partial \mLambda}{\partial \mLambda_{ij}})
\end{equation*}

$$
\mC = [\mX, \mZ]
\mW = \diag(f(\vmu, \mLambda))
\mLambda = \begin{bmatrix}
\mLambda_{11} & \mLambda_{12} &  &\\
\mLambda_{21} & \mLambda_{22} &  &\\
& & \ddots & \\
& & & \mLambda_{p \times p}
\end{bmatrix}
$$

\section{NR update}
\begin{align*}
\mLambda &\leftarrow (\mC^T \mW \mC + \mB)^{-1} \\
\vmu &\leftarrow \vmu + \mLambda \mC^T (\vy - \mB^{(1)}(\mC\vmu, \diag (\mC \mLambda \mC^T))) - \mB \vmu
\end{align*}

$$
\frac{\partial \log p (\vy;\vmu, \mLambda)}{\partial r_{ij}} = \half \tr \left ((\mLambda^{-1} - \mC^T \mW \mC - \mB) \frac{\partial \mLambda}{\partial r_{ij}} \right )
$$

\begin{align*}
\mLambda &= \mR^T \mR, \\
\mR &= \begin{bmatrix}
e^{r_{11}} & r_{12} & r_{13} & \dots & r_{1p} \\
& e^{r_{22}} & & & & \\
&  & \ddots & & & \\
&  & & & & e^{r_{pp}}\\
\end{bmatrix}
\end{align*}

Recall that
$$E_{ij} =
\begin{cases}
0 & i \ne j \\
1 & i = j
\end{cases}
$$

Consider the proposal that instead of $\mLambda = \mR^T \mR$, we choose
$\mLambda = (\mR^T \mR)^{-1}$. Then

\begin{align*}
\frac{\partial \log p(\vy; \vmu, \mLambda)}{\partial r_{ij}} &= - \half \tr \left( (\mLambda^{-1} - \mC^T \mW \mC - \mB) \times \mLambda \frac{\partial R^T R}{\partial r_{ij}} \mLambda \right) \\
&= - \half \tr \left( \mLambda(\mLambda^{-1} - \mC^T\mW\mC - B)\mLambda \times [(E_{ij} e^{I(i=j)r_{ij}})^T \mR + \mR^T E_{ij} e^{I(i=j) r_{ij}}] \right) \\
&= - \tr (\mR \mLambda (\mLambda^{-1} - \mC^T \mW \mC - \mB) \mLambda E_{ij})e^{I(i=j) r_{ij}} \\
&= - (\mR \mLambda (\mLambda^{-1} - \mC^T \mW \mC - \mB) \mLambda)_{ij} e^{I(i=j) r_{ij}} () \\
&= - (\mR^{-T} (\mLambda^{-1} - \mC^T \mW \mC - \mB) \mLambda)_{ij} e^{I(i=j) r_{ij}}
\end{align*}

as $\mLambda = (\mR^T \mR)^{-1} = \mR^{-1} \mR^{-T}$.

Here, I think $\mW = B^{(1)}(\vmu, \mLambda)$ and $\mB = \mSigma^{-1}$.

\section{Implementation}
Change the dmLambda line.

\section{Runtime efficiency}
$O(P^2 N - P^4)$ where $N=nm$, $P=p+m$.

$O(m + p + (m+p)^2) \to O((m + p + \frac{p(p-1)}{2} + p \times m))$

We will need to try the Newtown-Raphson approach as well.
\end{document}