\documentclass{amsart}
\title{Zero-inflated probability distributions}

\input{Definitions.tex}

\def\Var{\text{Var}}

\begin{document}

\maketitle

(1)

\begin{equation*}
\begin{array}{ll}
P(Y_i = 0) = p & \\
P(Y_j = y_i) = \left (\frac{1 - p}{1 - e^{-\lambda}}\right ) \frac{\lambda^{y_i} e^{-\lambda}}{y_i !} &, y_i \geq 1
\end{array}
\end{equation*}

rtp: $\sum_{i=0}^{\infty} P(Y_i = i) = 1$

\begin{equation*}
\begin{array}{lll}
\sum_{i=0}^{\infty} P(Y_i = i) &= p + \frac{1-p}{1 - e^{-\lambda}} \sum_{i=1}^{\infty} \frac{\lambda^{y_i} e^{-\lambda}}{y_i !} & \\
&= p + \frac{1 - p}{1 - e^{-\lambda}} (1 - e^{-\lambda}) &= 1
\end{array}
\end{equation*}

Expectation and variance
\begin{equation*}
\begin{array}{ll}
E(Y) &= \sum_{i=0}^{\infty} y_i P(Y_i = y_i) \\
&= 0 \times p + \sum_{i=1}^{\infty} i \left( \frac{1 - p}{1 - e^{-\lambda}} \right) \frac{\lambda^{y_i} e^{-\lambda}}{y_i !} \\
&= \left( \frac{1 - p}{1 - e^{-\lambda}} \right) \sum_{i=1}^{\infty} i \frac{\lambda^{y_i} e^{-\lambda}}{y_i !} \\
&= \left( \frac{1 - p}{1 - e^{-\lambda}} \right) (\lambda - e^{-\lambda})
\end{array}
\end{equation*}

$\Var(Y) = Y^2 - (EY)^2 \therefore E Y^2 = \Var Y + (E Y)^2$

\begin{equation*}
\begin{array}{lll}
E Y^2 &= \sum_{i=0}^{\infty} y^2 P(Y=i) & \\
&= y^2 P(Y=i) &= \sum_{i=1}^{\infty} y^2 \left( \frac{1 - p}{1 - e^{-\lambda}} \right) \frac{\lambda^{y_i} e^{-\lambda}}{y_i !} \\
&&= \left( \frac{1 - p}{1 - e^{-\lambda}} \right) \sum_{i=1}^{\infty}  y^2 \frac{\lambda^{y_i} e^{-\lambda}}{y_i !} \\
&&= \left( \frac{1 - p}{1 - e^{-\lambda}} \right) (\lambda + \lambda^2 - e^{-\lambda})
\end{array}
\end{equation*}

(2)

\begin{equation*}
\begin{array}{lll}
P(Y_i = 0) &= p + (1 - p) e^{-\lambda} & \\
P(Y_i = y_i) &= (1 - p) \frac{\lambda^{y_i} e^{-\lambda}}{y_i !}, & y_i \geq 1
\end{array}
\end{equation*}

(i) rtp: $\sum_{i=0}^{\infty} P(Y_i = i) = 1$
\begin{equation*}
\begin{array}{lll}
\sum_{i=0}^{\infty} P(Y_i = i) &= p + (1 - p) e^{-\lambda} + \sum_{i=1}^{\infty} (1 - p) \frac{\lambda^{y_i} e^{-\lambda}}{y_i !} \\
&= p + (1 - p) e^{-\lambda} + (1 - p) (1 - e^{-\lambda}) &= 1.
\end{array}
\end{equation*}

(ii)

\begin{equation*}
\begin{array}{lll}
E Y_i &= \sum_{i=0}^{\infty} i P(Y_i = i) &= \sum_{i=1}^{\infty} (1 - p) \frac{i \lambda^{y_i} e^{-\lambda}}{y_i !} \\
&&= (1 - p) \lambda
\end{array}
\end{equation*}

$\Var Y = E Y^2 - (E Y)^2 \Leftrightarrow E Y^2 = \Var Y + (E Y)^2$

\begin{equation*}
\begin{array}{lll}
E Y^2 &= \sum_{i=0}^\infty i^2 P(Y_i = i) &= \sum_{i=1}^\infty i^2 (1 - p) \frac{\lambda^{y_i} e^{-\lambda}}{y_i !} \\
&&= (1 - p) (\lambda + \lambda^2)
\end{array}
\end{equation*}

\end{document}